Some progress on graph promotion

Papers/Tree/TreeSnippets.thy
@@ -77,8 +77,104 @@ text_raw \<open>\Snip{graph-semantics-deterministic}
 \EndSnip\<close>
 
 definition graph_refinement :: "IRGraph \<Rightarrow> IRGraph \<Rightarrow> bool" where
-  "graph_refinement g1 g2 = (\<forall> n \<in> ids g1. 
-        (\<forall>m p v. ([g1, m, p] \<turnstile> n \<mapsto> v) \<longrightarrow> ([g2, m, p] \<turnstile> n \<mapsto> v)))"
+  "graph_refinement g1 g2 = 
+        (\<forall> n . n \<in> ids g1 \<longrightarrow> (\<forall>e1. (g1 \<turnstile> n \<triangleright> e1) \<longrightarrow> (\<exists>e2. (g2 \<turnstile> n \<triangleright> e2) \<and> e1 \<le> e2)))"
+
+lemma graph_refinement:
+  "graph_refinement g1 g2 \<Longrightarrow> (\<forall>n m p v. n \<in> ids g1 \<longrightarrow> ([g1, m, p] \<turnstile> n \<mapsto> v) \<longrightarrow> ([g2, m, p] \<turnstile> n \<mapsto> v))"
+  by (meson encodeeval_def graph_refinement_def le_expr_def)
+
+
+lemma mono_abs:
+  assumes "kind g1 n = AbsNode x \<and> kind g2 n = AbsNode x"
+  assumes "(g1 \<turnstile> x \<triangleright> xe1) \<and> (g2 \<turnstile> x \<triangleright> xe2)"
+  assumes "xe1 \<le> xe2"
+  assumes "(g1 \<turnstile> n \<triangleright> e1) \<and> (g2 \<turnstile> n \<triangleright> e2)"
+  shows "e1 \<le> e2"
+  by (metis AbsNode assms(1) assms(2) assms(3) assms(4) mono_unary repDet)
+
+lemma mono_not:
+  assumes "kind g1 n = NotNode x \<and> kind g2 n = NotNode x"
+  assumes "(g1 \<turnstile> x \<triangleright> xe1) \<and> (g2 \<turnstile> x \<triangleright> xe2)"
+  assumes "xe1 \<le> xe2"
+  assumes "(g1 \<turnstile> n \<triangleright> e1) \<and> (g2 \<turnstile> n \<triangleright> e2)"
+  shows "e1 \<le> e2"
+  by (metis NotNode assms(1) assms(2) assms(3) assms(4) mono_unary repDet)
+
+lemma mono_negate:
+  assumes "kind g1 n = NegateNode x \<and> kind g2 n = NegateNode x"
+  assumes "(g1 \<turnstile> x \<triangleright> xe1) \<and> (g2 \<turnstile> x \<triangleright> xe2)"
+  assumes "xe1 \<le> xe2"
+  assumes "(g1 \<turnstile> n \<triangleright> e1) \<and> (g2 \<turnstile> n \<triangleright> e2)"
+  shows "e1 \<le> e2"
+  by (metis NegateNode assms(1) assms(2) assms(3) assms(4) mono_unary repDet)
+
+lemma mono_logic_negation:
+  assumes "kind g1 n = LogicNegationNode x \<and> kind g2 n = LogicNegationNode x"
+  assumes "(g1 \<turnstile> x \<triangleright> xe1) \<and> (g2 \<turnstile> x \<triangleright> xe2)"
+  assumes "xe1 \<le> xe2"
+  assumes "(g1 \<turnstile> n \<triangleright> e1) \<and> (g2 \<turnstile> n \<triangleright> e2)"
+  shows "e1 \<le> e2"
+  by (metis LogicNegationNode assms(1) assms(2) assms(3) assms(4) mono_unary repDet)
+
+lemma mono_narrow:
+  assumes "kind g1 n = NarrowNode x \<and> kind g2 n = NarrowNode x"
+  assumes "stamp g1 n = stamp g2 n \<and> stamp g1 x = stamp g2 x"
+  assumes "(g1 \<turnstile> x \<triangleright> xe1) \<and> (g2 \<turnstile> x \<triangleright> xe2)"
+  assumes "xe1 \<le> xe2"
+  assumes "(g1 \<turnstile> n \<triangleright> e1) \<and> (g2 \<turnstile> n \<triangleright> e2)"
+  shows "e1 \<le> e2"
+  using assms mono_unary repDet NarrowNode
+  by metis
+
+lemma mono_sign_extend:
+  assumes "kind g1 n = SignExtendNode x \<and> kind g2 n = SignExtendNode x"
+  assumes "stamp g1 n = stamp g2 n \<and> stamp g1 x = stamp g2 x"
+  assumes "(g1 \<turnstile> x \<triangleright> xe1) \<and> (g2 \<turnstile> x \<triangleright> xe2)"
+  assumes "xe1 \<le> xe2"
+  assumes "(g1 \<turnstile> n \<triangleright> e1) \<and> (g2 \<turnstile> n \<triangleright> e2)"
+  shows "e1 \<le> e2"
+  by (metis SignExtendNode assms(1) assms(2) assms(3) assms(4) assms(5) mono_unary repDet)
+
+lemma mono_zero_extend:
+  assumes "kind g1 n = ZeroExtendNode x \<and> kind g2 n = ZeroExtendNode x"
+  assumes "stamp g1 n = stamp g2 n \<and> stamp g1 x = stamp g2 x"
+  assumes "(g1 \<turnstile> x \<triangleright> xe1) \<and> (g2 \<turnstile> x \<triangleright> xe2)"
+  assumes "xe1 \<le> xe2"
+  assumes "(g1 \<turnstile> n \<triangleright> e1) \<and> (g2 \<turnstile> n \<triangleright> e2)"
+  shows "e1 \<le> e2"
+  using assms mono_unary repDet ZeroExtendNode
+  by metis
+
+lemma mono_conditional:
+  assumes "kind g1 n = ConditionalNode c t f \<and> kind g2 n = ConditionalNode c t f"
+  assumes "(g1 \<turnstile> c \<triangleright> ce1) \<and> (g2 \<turnstile> c \<triangleright> ce2)"
+  assumes "(g1 \<turnstile> t \<triangleright> te1) \<and> (g2 \<turnstile> t \<triangleright> te2)"
+  assumes "(g1 \<turnstile> f \<triangleright> fe1) \<and> (g2 \<turnstile> f \<triangleright> fe2)"
+  assumes "ce1 \<le> ce2 \<and> te1 \<le> te2 \<and> fe1 \<le> fe2"
+  assumes "(g1 \<turnstile> n \<triangleright> e1) \<and> (g2 \<turnstile> n \<triangleright> e2)"
+  shows "e1 \<le> e2"
+  by (metis ConditionalNodeE IRNode.inject(6) assms(1) assms(2) assms(3) assms(4) assms(5) assms(6) mono_conditional repDet rep_conditional)
+
+lemma mono_add:
+  assumes "kind g1 n = AddNode x y \<and> kind g2 n = AddNode x y"
+  assumes "(g1 \<turnstile> x \<triangleright> xe1) \<and> (g2 \<turnstile> x \<triangleright> xe2)"
+  assumes "(g1 \<turnstile> y \<triangleright> ye1) \<and> (g2 \<turnstile> y \<triangleright> ye2)"
+  assumes "xe1 \<le> xe2 \<and> ye1 \<le> ye2"
+  assumes "(g1 \<turnstile> n \<triangleright> e1) \<and> (g2 \<turnstile> n \<triangleright> e2)"
+  shows "e1 \<le> e2"
+  using mono_binary assms
+  by (metis AddNodeE IRNode.inject(2) repDet rep_add)
+
+lemma mono_mul:
+  assumes "kind g1 n = MulNode x y \<and> kind g2 n = MulNode x y"
+  assumes "(g1 \<turnstile> x \<triangleright> xe1) \<and> (g2 \<turnstile> x \<triangleright> xe2)"
+  assumes "(g1 \<turnstile> y \<triangleright> ye1) \<and> (g2 \<turnstile> y \<triangleright> ye2)"
+  assumes "xe1 \<le> xe2 \<and> ye1 \<le> ye2"
+  assumes "(g1 \<turnstile> n \<triangleright> e1) \<and> (g2 \<turnstile> n \<triangleright> e2)"
+  shows "e1 \<le> e2"
+  using mono_binary assms
+  by (metis IRNode.inject(26) MulNodeE repDet rep_mul)
 
 text_raw \<open>\Snip{graph-refinement}
 \begin{center}
@@ -86,8 +182,8 @@ text_raw \<open>\Snip{graph-refinement}
 \end{center}
 \EndSnip\<close>
 
-definition as_set :: "IRGraph \<Rightarrow> (ID \<times> IRNode) set" where
-  "as_set g = {(n, kind g n) | n . n \<in> ids g}"
+definition as_set :: "IRGraph \<Rightarrow> (ID \<times> (IRNode \<times> Stamp)) set" where
+  "as_set g = {(n, kind g n, stamp g n) | n . n \<in> ids g}"
 
 (* hide as_set, should treat IRGraph as a set of pairs in paper *)
 translations
@@ -95,22 +191,286 @@ translations
 
 definition domain_subtraction :: "'a set \<Rightarrow> ('a \<times> 'b) set \<Rightarrow> ('a \<times> 'b) set"
   (infix "\<unlhd>" 30) where
-  "domain_subtraction s r = {(x, y) . (x, y) \<in> r | x \<notin> s}"
+  "domain_subtraction s r = {(x, y) . (x, y) \<in> r \<and> x \<notin> s}"
 
 notation (latex)
   domain_subtraction ("_ \<^latex>\<open>$\\ndres$\<close> _")
 
+
+lemma this_is_true:
+  assumes "n \<notin> ids g"
+  shows "\<not>(g \<turnstile> n \<triangleright> e)"
+proof -
+  have "kind g n = NoNode"
+    using assms ids_some by simp
+  show ?thesis
+  apply (rule notI)
+    apply (induct n e rule: rep.induct) apply auto
+    sorry
+qed
+
+lemma encodes_contains:
+  assumes "g \<turnstile> n \<triangleright> e"
+  shows "kind g n \<noteq> NoNode"
+  using assms apply (induction rule: rep.induct)
+  apply (metis IRNode.disc(349) is_ConstantNode_def)
+  using IRNode.distinct(2207) apply presburger
+  using IRNode.distinct(555) apply presburger
+  using IRNode.distinct(95) apply presburger
+  using IRNode.distinct(2141) apply presburger
+  using IRNode.distinct(2027) apply presburger
+  using IRNode.distinct(1635) apply presburger
+  using IRNode.distinct(191) apply presburger
+  using IRNode.distinct(1941) apply presburger
+  using IRNode.distinct(2405) apply presburger
+  using IRNode.distinct(285) apply presburger
+  using IRNode.distinct(2175) apply presburger
+  using IRNode.distinct(2441) apply presburger
+  using IRNode.distinct(1115) apply presburger
+  using IRNode.distinct(1187) apply presburger
+  using IRNode.distinct(1257) apply presburger
+  using IRNode.distinct(1985) apply presburger
+  using IRNode.distinct(2315) apply presburger
+  using IRNode.distinct(2445) apply presburger
+  by (metis is_preevaluated.simps(49))
+(*
+  using assms 
+proof -
+  fix n
+  assume "n \<notin> ids g"
+  then have "kind g n = NoNode"
+    using ids_some by simp
+  show "\<not>(g \<turnstile> n \<triangleright> e)"
+    apply (rule notI) apply (induct arbitrary: n e rule: rep.induct)
+  apply (rule notI)
+  apply (induct arbitrary: n e rule: rep.induct) apply auto
+proof -
+  fix n
+  show "kind g n = NoNode"
+qed
+  using ids_some assms sorry
+
+lemma unchanged_encoding:
+  assumes "\<forall>n \<in> (ids g1 - {n}). ([g1,m,p] \<turnstile> n \<mapsto> v) \<and> ([g2,m,p] \<turnstile> n \<mapsto> v)"
+  assumes "kind g1 n = kind g2 n"
+  assumes "stamp g1 n = stamp g2 n"
+  assumes "[g1,m,p] \<turnstile> n \<mapsto> v"
+  shows "[g2,m,p] \<turnstile> n \<mapsto> v"
+  using assms(4) unfolding encodeeval_def
+  using assms(1,2,3) sorry
+*)
+
+datatype ExprIRNode =
+  ExprUnaryNode IRUnaryOp ID |
+  ExprBinaryNode IRBinaryOp ID ID |
+  ExprConditionalNode ID ID ID |
+  ExprConstantNode Value |
+  ExprParameterNode nat |
+  ExprLeafNode ID |
+  NotExpr
+
+fun embed_expr :: "IRNode \<Rightarrow> ExprIRNode" where
+  "embed_expr (ConstantNode v) = ExprConstantNode v" |
+  "embed_expr (ParameterNode i) = ExprParameterNode i" |
+  "embed_expr (ConditionalNode c t f) = ExprConditionalNode c t f" |
+  "embed_expr (AbsNode x) = ExprUnaryNode UnaryAbs x" |
+  "embed_expr (NotNode x) = ExprUnaryNode UnaryNot x" |
+  "embed_expr (NegateNode x) = ExprUnaryNode UnaryNeg x" |
+  "embed_expr (LogicNegationNode x) = ExprUnaryNode UnaryLogicNegation x" |
+  "embed_expr (AddNode x y) = ExprBinaryNode BinAdd x y" |
+  "embed_expr (MulNode x y) = ExprBinaryNode BinMul x y" |
+  "embed_expr (SubNode x y) = ExprBinaryNode BinSub x y" |
+  "embed_expr (AndNode x y) = ExprBinaryNode BinAnd x y" |
+  "embed_expr (OrNode x y) = ExprBinaryNode BinOr x y" |
+  "embed_expr (XorNode x y) = ExprBinaryNode BinXor x y" |
+  "embed_expr (IntegerBelowNode x y) = ExprBinaryNode BinIntegerBelow x y" |
+  "embed_expr (IntegerEqualsNode x y) = ExprBinaryNode BinIntegerEquals x y" |
+  "embed_expr (IntegerLessThanNode x y) = ExprBinaryNode BinIntegerLessThan x y" |
+(*
+  "embed_expr (NarrowNode x) = ExprUnaryNode (UnaryNarrow 0 0) x" |
+  "embed_expr (SignExtendNode x) = ExprUnaryNode (UnarySignExtend 0 0) x" |
+  "embed_expr (ZeroExtendNode x) = ExprUnaryNode (UnaryZeroExtend 0 0) x" |
+*)
+  "embed_expr _ = NotExpr"
+
+definition is_convert_node :: "IRNode \<Rightarrow> bool" where
+  "is_convert_node n = ((is_NarrowNode n) \<or> (is_SignExtendNode n) \<or> (is_ZeroExtendNode n))"
+
+lemmas reps =
+  rep_constant
+  rep_parameter
+  rep_conditional
+  rep_abs
+  rep_not
+  rep_negate
+  rep_logicnegation
+  rep_add
+  rep_sub
+  rep_mul
+  rep_and
+  rep_or
+  rep_xor
+  rep_integer_below
+  rep_integer_equals
+  rep_integer_less_than
+  rep_narrow
+  rep_sign_extend
+  rep_zero_extend
+  rep_load_field
+
+lemma unary_embed:
+  assumes "g \<turnstile> n \<triangleright> UnaryExpr op x"
+  assumes "\<not>(is_convert_node (kind g n))"
+  shows "\<exists> x' . embed_expr (kind g n) = ExprUnaryNode op x'"
+  using assms apply (induction "UnaryExpr op x" rule: rep.induct; simp)
+  unfolding is_convert_node_def
+  using is_NarrowNode_def is_SignExtendNode_def is_ZeroExtendNode_def by blast+
+
+lemma equal_embedded_x:
+  assumes "g \<turnstile> n \<triangleright> UnaryExpr op xe"
+  assumes "embed_expr (kind g n) = ExprUnaryNode op' x"
+  shows "g \<turnstile> x \<triangleright> xe"
+  using assms by (induction "UnaryExpr op xe" rule: rep.induct; simp)
+
+lemma blah:
+  assumes "embed_expr (kind g n) = ExprUnaryNode op n'"
+  assumes "g \<turnstile> n' \<triangleright> e"
+  shows "(g \<turnstile> n \<triangleright> UnaryExpr op e)"
+  using assms(2,1) apply (cases "kind g n"; auto)
+  using rep.AbsNode apply blast
+  using rep.LogicNegationNode apply blast
+  using rep.NegateNode apply blast
+  using rep.NotNode by blast
+
+lemma not_excluded_keep_type:
+  assumes "n \<in> ids g1"
+  assumes "n \<notin> excluded"
+  assumes "(excluded \<unlhd> as_set g1) \<subseteq> as_set g2"
+  shows "kind g1 n = kind g2 n \<and> stamp g1 n = stamp g2 n"
+  using assms unfolding as_set_def domain_subtraction_def by blast
+
+lemma graph_semantics_preservation:
+  assumes a: "e1' \<le> e2'"
+  assumes b: "({n'} \<unlhd> as_set g1) \<subseteq> as_set g2"
+  assumes c: "g1 \<turnstile> n' \<triangleright> e1'"
+  assumes d: "g2 \<turnstile> n' \<triangleright> e2'"
+  assumes hack: "(\<forall> n. n \<in> ids g1 \<longrightarrow> \<not>(is_convert_node (kind g1 n)))"
+  shows "graph_refinement g1 g2"
+  unfolding graph_refinement_def 
+  apply (rule allI) apply (rule impI) apply (rule allI) apply (rule impI)
+proof -
+  fix n e1
+  assume e: "n \<in> ids g1"
+  assume f: "(g1 \<turnstile> n \<triangleright> e1)"
+
+  show "\<exists> e2. (g2 \<turnstile> n \<triangleright> e2) \<and> e1 \<le> e2"
+  proof (cases "n = n'")
+    case True
+    have g: "e1 = e1'" using c f True repDet by simp
+    have h: "(g2 \<turnstile> n \<triangleright> e2') \<and> e1' \<le> e2'"
+      using True a d by blast
+    then show ?thesis 
+      using g by blast
+  next
+    case False
+    have "n \<notin> {n'}"
+      using False by simp
+    then have i: "kind g1 n = kind g2 n \<and> stamp g1 n = stamp g2 n"
+      using not_excluded_keep_type
+      using b e by presburger
+    show ?thesis using f
+      proof (cases e1)
+        case (UnaryExpr op xe1)
+        from UnaryExpr have k: "g1 \<turnstile> n \<triangleright> UnaryExpr op xe1" using f by blast
+        have "\<not>(is_convert_node (kind g1 n))"
+          using hack encodes_contains ids_some
+          using e by blast
+        then obtain xn where l: "embed_expr (kind g1 n) = ExprUnaryNode op xn"
+          using k using unary_embed
+          by blast
+        then have kk: "g1 \<turnstile> xn \<triangleright> xe1"
+          using repDet k equal_embedded_x by blast
+        then show ?thesis
+        proof (cases "xn = n'")
+          case True
+          then have n: "xe1 = e1'" using c UnaryExpr repDet l
+            using kk by presburger
+          have r: "UnaryExpr op e1' \<le> UnaryExpr op e2'"
+            using a mono_unary by simp
+          have "g2 \<turnstile> n \<triangleright> UnaryExpr op e2'" using i k UnaryExpr n d True
+            using blah
+            using l by presburger
+          then show ?thesis
+            using r UnaryExpr n by blast 
+        next
+          case False
+          then have "g1 \<turnstile> xn \<triangleright> xe1" using UnaryExpr
+            by (simp add: kk)
+          then have "\<exists> xe2. (g2 \<turnstile> xn \<triangleright> xe2) \<and> xe1 \<le> xe2" sorry
+          then have "\<exists> xe2. (g2 \<turnstile> n \<triangleright> UnaryExpr op xe2) \<and> UnaryExpr op xe1 \<le> UnaryExpr op xe2"
+            by (metis blah i l mono_unary)
+          then show ?thesis
+            using UnaryExpr by blast
+        qed
+      next
+        case (BinaryExpr x1 e11 e12)
+        then show ?thesis sorry
+      next
+        case (ConditionalExpr e11 e12 e13)
+        then show ?thesis sorry
+      next
+        case (ConstantExpr x)
+        then show ?thesis sorry
+      next
+        case (ParameterExpr x1 x2)
+        then show ?thesis sorry
+      next
+        case (LeafExpr x1 x2)
+        then show ?thesis sorry
+      qed
+  qed
+qed
+
+(*
 lemma graph_semantics_preservation:
   "e1 \<le> e2 \<and> (g1 \<turnstile> n \<triangleright> e1) \<and> (g2 \<turnstile> n \<triangleright> e2) \<and> (({n} \<unlhd> as_set g1) \<subseteq> as_set g2) \<Longrightarrow>
-     graph_refinement g1 g2"
-  unfolding domain_subtraction_def as_set_def
-proof (cases "n \<in> ids g")
+     graph_refinement g1 g2" (is "?asm \<Longrightarrow> ?con")
+proof (cases "n \<in> ids g1")
   case True
-  then show ?thesis  sorry
+  assume a: ?asm
+  show ?thesis
+    unfolding graph_refinement_def
+  proof ((rule allI)+; (rule impI)+)
+    fix n1 m p v
+    assume a0: "n1 \<in> ids g1"
+    assume a1: "([g1,m,p] \<turnstile> n1 \<mapsto> v)"
+    obtain e1 where "g1 \<turnstile> n1 \<triangleright> e1"
+      using a1 encodeeval_def by auto
+    have same: "n1 \<notin> {n} \<Longrightarrow> kind g1 n1 = kind g2 n1 \<and> stamp g1 n1 = stamp g2 n1"
+      using a a0 unfolding as_set_def domain_subtraction_def
+      by blast
+    show "([g2,m,p] \<turnstile> n1 \<mapsto> v)" using a0 a1 a unfolding encodeeval_def
+      apply (cases "n = n1")
+      using a1 encodeeval_def le_expr_def repDet apply blast
+      using same unchanged_encoding sorry
+  qed
 next
   case False
-  then show ?thesis sorry
+  assume a: ?asm
+  show ?thesis (* using False unfolding graph_refinement_def as_set_def domain_subtraction_def *)
+    unfolding graph_refinement_def
+  proof ((rule allI)+; (rule impI)+)
+    fix n m p v
+    assume a0: "n \<in> ids g1"
+    assume a1: "([g1,m,p] \<turnstile> n \<mapsto> v)"
+    have "\<not>(\<exists>e. (g1 \<turnstile> n \<triangleright> e))"
+      using this_is_true
+      by (meson False a)
+    then show "([g2,m,p] \<turnstile> n \<mapsto> v)" using a0 a1 a unfolding encodeeval_def
+      by blast
+  qed
 qed
+*)
 
 
 text_raw \<open>\Snip{graph-semantics-preservation}
